complete proof up to acceptors send2b

ironfleet/src/Dafny/Distributed/Protocol/RSL/FailureProof/Phase2Proof.i.dfy
@@ -18,27 +18,27 @@ import opened CommonProof__Constants_i
 *****************************************************************************************/
 
 /* Main performance guarantee for phase 2 post-failure */
-predicate PerformanceGuarantee(ts:TimestampedRslState, opn:OperationNumber){
+predicate PerformanceGuarantee(ts:TimestampedRslState, opn:OperationNumber)
+    requires |ts.t_replicas| > 2
+    requires RslConsistency(ts)
+{
     && PerformanceGuarantee_Response(ts)
     && PerformanceGuarantee_2b(ts, opn)
     && PerformanceGuarantee_2a(ts, opn)
 }
 
-predicate PerformanceGuarantee_Response(ts:TimestampedRslState) {
-    // 0 < |ts.constants.config.replica_ids|
-    //     && (forall pkt :: 
-    //             && pkt in ts.undeliveredPackets
-    //             && pkt.msg.v.RslMessage_Reply?
-    //             && pkt.src == ts.constants.config.replica_ids[0]
-    //             ==>
-    //             TimeLe(pkt.msg.ts, TimeBoundReply(req_time, ts.constants))
-    //     )
-    //TODO
-    true
+predicate PerformanceGuarantee_Response(ts:TimestampedRslState) 
+    requires |ts.t_replicas| > 2
+    requires RslConsistency(ts)
+{
+    forall pkt | 
+        && pkt in ts.undeliveredPackets 
+        && IsNewReplyPacket(ts, pkt)
+    :: TimeLe(pkt.msg.ts, TimeBoundReplyFailure())
 }
 
 predicate PerformanceGuarantee_2b(ts:TimestampedRslState, opn:OperationNumber) {
-    forall pkt {:trigger pkt.msg.v.RslMessage_2a?} | 
+    forall pkt {:trigger pkt.msg.v.RslMessage_2b?} | 
         && pkt in ts.undeliveredPackets 
         && IsNew2aPacket(pkt, opn)
     :: TimeLe(pkt.msg.ts, TimeBound2bDeliveryPost())
@@ -59,22 +59,35 @@ function TimeBound2bDeliveryPost() : Timestamp {
     TimeBound2aDeliveryPost() + ProcessPacket + MaxQueueTime + D
 }
 
+function TimeBoundPhase2LeaderPost(nextActionIndex:int) : Timestamp
+    requires 0 <= nextActionIndex < 10
+{
+  TimeBound2bDeliveryPost() + MaxQueueTime + TimeActionRange(nextActionIndex)
+}
+
+function TimeBoundReplyFailure() : Timestamp {
+    TimeBoundPhase2LeaderPost(7) + D
+}
+
 /*****************************************************************************************
 *                                     Assumptions                                        *
 *****************************************************************************************/
 
 /* Conjunction of all assumptions */
-predicate RslAssumption(ts:TimestampedRslState)
+predicate RslAssumption(ts:TimestampedRslState, opn:OperationNumber)
 {
-    && RelationsAssumptions()
     && RslConsistency(ts)
     && NoPacketDuplication(ts)
     && |ts.t_replicas| > 2  // For failure to be meaningful
     && ts.constants.params.max_batch_size == 1
 
     && (var nextStep := ts.t_environment.nextStep; 
-    nextStep.LEnvStepHostIos? ==>
-    (forall io | io in nextStep.ios && io.LIoOpReceive? :: !io.r.msg.v.RslMessage_Heartbeat? && !io.r.msg.v.RslMessage_Request?))
+        && nextStep.LEnvStepHostIos? ==>
+            && (forall io | io in nextStep.ios :: !io.LIoOpTimeoutReceive?)
+            && (forall io | io in nextStep.ios && io.LIoOpReceive? :: !io.r.msg.v.RslMessage_Heartbeat? && !io.r.msg.v.RslMessage_Request? && !io.r.msg.v.RslMessage_AppStateSupply?)
+    )
+    && NewLeaderDoesNotReceiveOld2b(ts)
+    && NewLeaderDoesNotProposeFurtherOps(ts, opn)
     && LeaderAlwaysOne(ts)
     && minD < SelfDelivery < D < 2*minD
     && ProcessPacket > 0
@@ -84,8 +97,19 @@ predicate RslAssumption(ts:TimestampedRslState)
     && BoundedQueueingAssumption(ts)
 }
 
-predicate RelationsAssumptions() {
-    && TimeLe(req_time, NewLeaderInitTS)
+predicate NewLeaderDoesNotProposeFurtherOps(ts:TimestampedRslState, opn:OperationNumber) 
+    requires |ts.t_replicas| > 2 
+{
+    ts.t_replicas[1].v.replica.proposer.constants.all.params.max_integer_val == UpperBoundFinite(opn + 1)
+}
+
+/* Assume that the leader does not receive leftover 2b packets from before leader election */
+predicate NewLeaderDoesNotReceiveOld2b(ts:TimestampedRslState) 
+    requires |ts.t_replicas| > 2 
+{
+    var nextStep := ts.t_environment.nextStep;
+    nextStep.LEnvStepHostIos? ==>
+    (forall io | io in nextStep.ios && io.LIoOpReceive? && io.r.msg.v.RslMessage_2b? :: io.r.msg.v.bal_2b != Ballot(1, 0))
 }
 
 predicate LeaderAlwaysOne(ts:TimestampedRslState) 
@@ -139,28 +163,28 @@ ghost const req_time:Timestamp
 /* Initial timestamp of replica 1 */
 ghost const NewLeaderInitTS:Timestamp
 
-//  Invariant of starting state of Phase2 proof
-predicate BoundaryCond(ts:TimestampedRslState, opn:OperationNumber) 
-    requires |ts.t_replicas| > 2
-{
-    && BoundaryCond_ExistingPacketsBallot(ts)
-    && BoundaryCond_NewLeader(ts, opn)
-}
+// //  Invariant of starting state of Phase2 proof
+// predicate BoundaryCond(ts:TimestampedRslState, opn:OperationNumber) 
+//     requires |ts.t_replicas| > 2
+// {
+//     && BoundaryCond_ExistingPacketsBallot(ts)
+//     && BoundaryCond_NewLeader(ts, opn)
+// }
 
 
-predicate BoundaryCond_NewLeader(ts:TimestampedRslState, opn:OperationNumber) 
-    requires |ts.t_replicas| > 2
-{
-    var r := ts.t_replicas[1].v.replica;
-    && ts.t_replicas[1].v.nextActionIndex == 3
-    && r.proposer.current_state == 2
-    && r.proposer.election_state.current_view == Ballot(1, 1)
-    && r.proposer.max_ballot_i_sent_1a == Ballot(1, 1)
-    && opn == r.proposer.next_operation_number_to_propose
-    && opn == r.executor.ops_complete
-    && LeaderSet1bContainsRequest(ts)
-    && ts.t_replicas[1].v.replica.proposer.request_queue == []
-}
+// predicate BoundaryCond_NewLeader(ts:TimestampedRslState, opn:OperationNumber) 
+//     requires |ts.t_replicas| > 2
+// {
+//     var r := ts.t_replicas[1].v.replica;
+//     && ts.t_replicas[1].v.nextActionIndex == 3
+//     && r.proposer.current_state == 2
+//     && r.proposer.election_state.current_view == Ballot(1, 1)
+//     && r.proposer.max_ballot_i_sent_1a == Ballot(1, 1)
+//     && opn == r.proposer.next_operation_number_to_propose
+//     && opn == r.executor.ops_complete
+//     && LeaderSet1bContainsRequest(ts)
+//     && ts.t_replicas[1].v.replica.proposer.request_queue == []
+// }
 
 predicate LeaderSet1bContainsRequest(ts:TimestampedRslState) 
     requires |ts.t_replicas| > 2
@@ -171,28 +195,28 @@ predicate LeaderSet1bContainsRequest(ts:TimestampedRslState)
 }
 
 
-predicate BoundaryCond_ExistingPacketsBallot(ts:TimestampedRslState) {
-    forall pkt | pkt in ts.undeliveredPackets :: Boundary_ExistingPacketsBallot(pkt)
-}
-predicate Boundary_ExistingPacketsBallot(pkt:TimestampedLPacket<EndPoint, RslMessage>) {
-    match pkt.msg.v {
-        // All 1a and 1b packets have Ballot (1, 1)
-        case RslMessage_1a(bal_1a)              => bal_1a == Ballot(1, 1) 
-        case RslMessage_1b(bal_1b,_,_)          => bal_1b == Ballot(1, 1) 
-        // All 2a and 2b messages have Ballot(1, 0)
-        case RslMessage_2a(bal_2a,_,_)          => bal_2a == Ballot(1, 0)
-        case RslMessage_2b(bal_2b,_,_)          => bal_2b == Ballot(1, 0)
+// predicate BoundaryCond_ExistingPacketsBallot(ts:TimestampedRslState) {
+//     forall pkt | pkt in ts.undeliveredPackets :: Boundary_ExistingPacketsBallot(pkt)
+// }
+// predicate Boundary_ExistingPacketsBallot(pkt:TimestampedLPacket<EndPoint, RslMessage>) {
+//     match pkt.msg.v {
+//         // All 1a and 1b packets have Ballot (1, 1)
+//         case RslMessage_1a(bal_1a)              => bal_1a == Ballot(1, 1) 
+//         case RslMessage_1b(bal_1b,_,_)          => bal_1b == Ballot(1, 1) 
+//         // All 2a and 2b messages have Ballot(1, 0)
+//         case RslMessage_2a(bal_2a,_,_)          => bal_2a == Ballot(1, 0)
+//         case RslMessage_2b(bal_2b,_,_)          => bal_2b == Ballot(1, 0)
 
-        // Cases where I don't care
-        case RslMessage_Heartbeat(_,_,_)        => true
-        case RslMessage_Invalid                 => true
-        case RslMessage_Request(_,_)            => true
-        case RslMessage_Reply(_,_)              => true
-        case RslMessage_AppStateRequest(_,_)    => true
-        case RslMessage_AppStateSupply(_,_,_,_) => true
-        case RslMessage_StartingPhase2(_,_)     => true
-    }
-}
+//         // Cases where I don't care
+//         case RslMessage_Heartbeat(_,_,_)        => true
+//         case RslMessage_Invalid                 => true
+//         case RslMessage_Request(_,_)            => true
+//         case RslMessage_Reply(_,_)              => true
+//         case RslMessage_AppStateRequest(_,_)    => true
+//         case RslMessage_AppStateSupply(_,_,_,_) => true
+//         case RslMessage_StartingPhase2(_,_)     => true
+//     }
+// }
 
 
 
@@ -210,7 +234,7 @@ predicate RslPerfInvariant(ts:TimestampedRslState, opn:OperationNumber)
     requires |ts.t_replicas| > 2
 {
     && RslConsistency(ts)
-    && AlwaysInvariant(ts)
+    && AlwaysInvariant(ts, opn)
     && PerformanceGuarantee(ts, opn)
     && PacketsBallotInvariant(ts)
     && (|| Before_2a_Sent_Invariant(ts, opn)
@@ -231,7 +255,7 @@ predicate RequestBatchSrcInClientIds(ts:TimestampedRslState, v:RequestBatch)
   forall r :: r in v ==> r.client in ts.constants.config.clientIds
 }
 
-predicate AlwaysInvariant(ts:TimestampedRslState)
+predicate AlwaysInvariant(ts:TimestampedRslState, opn:OperationNumber)
     requires |ts.t_replicas| > 2
 {
     && ServersAreNotClients(ts)
@@ -248,7 +272,7 @@ predicate AlwaysInvariant(ts:TimestampedRslState)
             )
         && (ts.t_replicas[idx].v.replica.executor.next_op_to_execute.OutstandingOpKnown?
             ==> RequestBatchSrcInClientIds(ts, ts.t_replicas[idx].v.replica.executor.next_op_to_execute.v)
-    )
+        )
     )
 }
 
@@ -278,14 +302,32 @@ predicate ExistingPacketsBallot(pkt:TimestampedLPacket<EndPoint, RslMessage>) {
     }
 }
 
+
+predicate All2aPackets_BalLeq_Opn(ts:TimestampedRslState, ballot:Ballot, opn:OperationNumber) {
+    forall pkt | pkt in ts.t_environment.sentPackets && pkt.msg.v.RslMessage_2a?
+    ::  && BalLeq(pkt.msg.v.bal_2a, ballot)
+        && pkt.msg.v.opn_2a == opn
+}
+
+predicate All2bPackets_BalLeq_Opn(ts:TimestampedRslState, ballot:Ballot, opn:OperationNumber) {
+    forall pkt | pkt in ts.t_environment.sentPackets && pkt.msg.v.RslMessage_2b?
+    ::  && BalLeq(pkt.msg.v.bal_2b, ballot)
+        && pkt.msg.v.opn_2b == opn
+}
+
 // Things that are true before 2a packets are sent out by the leader
 predicate Before_2a_Sent_Invariant(ts:TimestampedRslState, opn:OperationNumber) 
     requires |ts.t_replicas| > 2
+    requires RslConsistency(ts)
 {
     var l := ts.t_replicas[1];
     var r := l.v.replica;
+    && All2aPackets_BalLeq_Opn(ts, Ballot(1, 0), opn)
+    && All2bPackets_BalLeq_Opn(ts, Ballot(1, 0), opn)
     && (!exists pkt :: pkt in ts.t_environment.sentPackets && IsNew2aPacket(pkt, opn))
     && (!exists pkt :: pkt in ts.t_environment.sentPackets && IsNew2bPacket(pkt, opn))
+    && (!exists pkt :: pkt in ts.t_environment.sentPackets && IsNewReplyPacket(ts, pkt))
+    && PerformanceGuarantee_Response(ts)
     && TimeLe(l.ts, NewLeaderInitTS)     // leader timestamp
     && l.v.nextActionIndex == 3          // leader action index is 3
     && LeaderSet1bContainsRequest(ts)
@@ -294,32 +336,86 @@ predicate Before_2a_Sent_Invariant(ts:TimestampedRslState, opn:OperationNumber)
     && r.proposer.election_state.current_view == Ballot(1, 1)
     && r.proposer.max_ballot_i_sent_1a == Ballot(1, 1)
     && opn == r.proposer.next_operation_number_to_propose
+    
+    // Learner and Executor states
+    && opn == r.executor.ops_complete
+    && r.learner.unexecuted_learner_state == map[]
+    && r.executor.next_op_to_execute == OutstandingOpUnknown()
+    && BalLt(r.learner.max_ballot_seen, Ballot(1, 1))
 }
 
 // Things that are true after 2a packets are sent out by the leader
 predicate Before_2b_Sent_Invariant(ts:TimestampedRslState, opn:OperationNumber) 
     requires |ts.t_replicas| > 2
+    requires RslConsistency(ts)
 {
     var l := ts.t_replicas[1];
     var r := l.v.replica;
+    && All2aPackets_BalLeq_Opn(ts, Ballot(1, 1), opn)
+    && All2bPackets_BalLeq_Opn(ts, Ballot(1, 0), opn)
     && (exists pkt :: pkt in ts.t_environment.sentPackets && IsNew2aPacket(pkt, opn))
     && (!exists pkt :: pkt in ts.t_environment.sentPackets && IsNew2bPacket(pkt, opn))
+    && (!exists pkt :: pkt in ts.t_environment.sentPackets && IsNewReplyPacket(ts, pkt))
     && PerformanceGuarantee_2a(ts, opn)
-    && r.proposer.current_state == 2
+    && PerformanceGuarantee_Response(ts)
     && 0 <= ts.t_replicas[1].v.nextActionIndex <= 9
+    && r.proposer.current_state == 2
     && r.proposer.next_operation_number_to_propose > opn
+
+    // Learner and Executor states
+    && r.learner.unexecuted_learner_state == map[]
+    && (forall opn' | opn' in r.learner.unexecuted_learner_state :: opn' == opn)
+    && opn == r.executor.ops_complete
+    && r.executor.next_op_to_execute == OutstandingOpUnknown()
+    && BalLt(r.learner.max_ballot_seen, Ballot(1, 1))
 }
 
 predicate After_2b_Sent_Invariant(ts:TimestampedRslState, opn:OperationNumber) 
     requires |ts.t_replicas| > 2
+    requires RslConsistency(ts)
 {
     var l := ts.t_replicas[1];
     var r := l.v.replica;
-    && exists pkt :: pkt in ts.t_environment.sentPackets && IsNew2bPacket(pkt, opn)
+    && All2aPackets_BalLeq_Opn(ts, Ballot(1, 1), opn)
+    && All2bPackets_BalLeq_Opn(ts, Ballot(1, 1), opn)
+    && (exists pkt :: pkt in ts.t_environment.sentPackets && IsNew2bPacket(pkt, opn))
     && PerformanceGuarantee_2a(ts, opn)
     && PerformanceGuarantee_2b(ts, opn)
+    && PerformanceGuarantee_Response(ts)
+    && 0 <= ts.t_replicas[1].v.nextActionIndex <= 9
     && r.proposer.current_state == 2
     && r.proposer.next_operation_number_to_propose > opn
+
+    // Learner and Executor states
+    && opn == r.executor.ops_complete
+    && r.executor.next_op_to_execute == OutstandingOpUnknown()
+    && BalLeq(r.learner.max_ballot_seen, Ballot(1, 1))
+
+    && Get2bCount(r, opn, Ballot(1, 1)) <= LMinQuorumSize(ts.constants.config)
+
+    && (Get2bCount(r, opn, Ballot(1, 1)) < LMinQuorumSize(ts.constants.config)
+    ==> r.executor.next_op_to_execute.OutstandingOpUnknown?)
+
+    && (Get2bCount(r, opn, Ballot(1, 1)) == LMinQuorumSize(ts.constants.config)
+    ==> TimeLe(l.ts, TimeBoundPhase2LeaderPost(l.v.nextActionIndex)))
+
+    && (l.v.nextActionIndex == 6
+        && Get2bCount(r, opn, Ballot(1, 1)) == LMinQuorumSize(ts.constants.config)
+        ==> 
+        r.executor.next_op_to_execute.OutstandingOpKnown?
+    )
+
+    && (r.executor.next_op_to_execute.OutstandingOpKnown?
+    ==> Get2bCount(r, opn, Ballot(1, 1)) == LMinQuorumSize(ts.constants.config)
+    )
+
+    && (forall opn' | opn' in r.learner.unexecuted_learner_state :: opn' == opn)
+
+    && (opn in r.learner.unexecuted_learner_state 
+        ==>
+        && r.learner.max_ballot_seen == Ballot(1, 1)
+        && (forall id :: id in r.learner.unexecuted_learner_state[opn].received_2b_message_senders ==> id in ts.constants.config.replica_ids)
+    )
 }
 
 
@@ -339,6 +435,23 @@ predicate IsNew2bPacket(pkt:TimestampedRslPacket, opn:OperationNumber) {
     && pkt.msg.v.RslMessage_2b?
     && pkt.msg.v.bal_2b == Ballot(1, 1)
     && pkt.msg.v.opn_2b == opn
+}
+
+predicate IsNewReplyPacket(ts:TimestampedRslState, pkt:TimestampedRslPacket) 
+    requires |ts.t_replicas| > 2
+    requires RslConsistency(ts)
+{
+    && pkt.msg.v.RslMessage_Reply?
+    && pkt.src == ts.constants.config.replica_ids[1]
+}
+
+function Get2bCount(s:LReplica, opn:OperationNumber, ballot:Ballot) : int
+{
+    if s.learner.max_ballot_seen != ballot then 0 else
+  if opn !in s.learner.unexecuted_learner_state then
+    0
+  else
+    |s.learner.unexecuted_learner_state[opn].received_2b_message_senders|
 }
 
 }
